\begin{enumerate}[label=\thesection.\arabic*.,ref=\thesection.\theenumi]
\numberwithin{equation}{enumi}
\item
The response of the system
\begin{align}
     G(s)= \frac{s-2}{(s+1)(s+3)} ,
\end{align} 
to the unit step input u(t) is y(t). The value of \(\frac{dy}{dt}\) at t=0^+ is:

\\
\solution 
Input of the system is u(t),
We know that, 

 \begin{align}
    Y(s) &= X(s).H(s) = \sbrak{\frac{1}{s}}\sbrak{\frac{s-2}{(s+1)(s+3)}}
    \\
    &= \frac{s-2}{s(s+1)(s+3)}
    \\
    &= \frac{-2}{3s} + \frac{3}{2(s+1)} + \frac{-5}{6(s+3)}
 \end{align}

Applying the inverse laplace transform , we get:

 \begin{align}
    c(t) &= L^{-1} \sbrak{ \frac{1}{s}} - L^{-1}\sbrak{\frac{1}{1+s}} - L^{-1}\sbrak{\frac{1}{(1+s)^2}} 
    \\
    &= \brak{\frac{-2}{3} + \frac{3}{2}e^{-t} - \frac{5}{6}e^{-3t}}  u(t)
    \label{eq:sec_order_op}
 \end{align}

On differentiating it we get,
 \begin{align}
    \frac{dy(t)}{dt} = \frac{-3}{2}e^-^t + \frac{5}{2}e^-^3^t
 \end{align}
At t = 0^+
 
 \begin{align}
    \frac{dy(0^+)}{dt} = \frac{-3}{2} + \frac{5}{2} = 1
 \end{align}



\end{enumerate}
    

